concrete

ByteArray.v
@@ -91,52 +91,47 @@ Definition valid_memory (mem : Memory) : Prop :=
   (* arrays stay within their address ranges *)
   ((all_array_offsets_valid mem) = true).
 
-(* a pointer is an offset into an array *)
-Inductive Ptr : Type :=
-| Address (base: nat) (offset : nat).
-Definition ptr_base (p : Ptr) : positive :=
-  idx_to_key match p with
-  | Address x _ => x
-  end.
-Definition ptr_off (p : Ptr) : positive :=
-  idx_to_key match p with
-  | Address _ x => x
-  end.
+Definition uint_to_pos (u : uintptr) : positive :=
+  Pos.of_nat ((Z.to_nat (unsigned u)) + 1).
 
 (* check if a pointer's array is in memory *)
-Definition find_array (mem : Memory) (p : Ptr) : option Array :=
-  mem !! (ptr_base p).
+Definition find_array (mem : Memory) (base : uintptr) : option Array :=
+  mem !! (uint_to_pos base).
 
 (* load the value that a pointer points to *)
-Definition ld_arr (a : Array) (p : Ptr) : option uint8 :=
-  (bytes a) !! (ptr_off p).
-Definition ld_mem (mem : Memory) (p : Ptr) : option uint8 :=
-  match (find_array mem p) with
-  | Some a => ld_arr a p
+Definition ld_arr (a : Array) (offset : uintptr) : option uint8 :=
+  let offset' := uint_to_pos offset in
+  if (Pos.ltb offset' (Pos.of_nat (len a))) then
+     (bytes a) !! offset'
+  else
+    None.
+Definition ld_mem (mem : Memory) (base : uintptr) (offset : uintptr) : option uint8 :=
+  match (find_array mem base) with
+  | Some a => ld_arr a offset
   | None => None
   end.
 
 (* store a value into a pointer *)
-Definition st_arr (a : Array) (p : Ptr) (v : uint8) : option Array :=
-  let off := ptr_off p in
-  if (Pos.ltb off (Pos.of_nat (len a))) then
+Definition st_arr (a : Array) (offset : uintptr) (v : uint8) : option Array :=
+  let offset' := uint_to_pos offset in
+  if (Pos.ltb offset' (Pos.of_nat (len a))) then
     Some {|
       base := base a;
       len := len a;
-      bytes := PMap.set off (Some v) (bytes a)
+      bytes := PMap.set offset' (Some v) (bytes a)
     |}
   else
     None.
-Definition st_mem' (mem : Memory) (p : Ptr) (v : uint8) : option Memory :=
-  match (find_array mem p) with
-  | Some a => match (st_arr a p v) with
-    | Some a' => Some (PMap.set (ptr_base p) (Some a') mem)
+Definition st_mem' (mem : Memory) (base : uintptr) (offset : uintptr) (v : uint8) : option Memory :=
+  match (find_array mem base) with
+  | Some a => match (st_arr a offset v) with
+    | Some a' => Some (PMap.set (uint_to_pos base) (Some a') mem)
     | None => None
     end
   | None => None
   end.
-Definition st_mem (mem : Memory) (p : Ptr) (v : uint8) : Memory :=
-  match (st_mem' mem p v) with
+Definition st_mem (mem : Memory) (base : uintptr) (offset : uintptr) (v : uint8) : Memory :=
+  match (st_mem' mem base offset v) with
   | Some mem' => mem'
   | None => mem
   end.
@@ -144,211 +139,436 @@ Definition st_mem (mem : Memory) (p : Ptr) (v : uint8) : Memory :=
 (* accessing a pointer is valid if...
   - there exists an associated array in memory
   - the pointer's access into that array is in-bounds *)
-Definition mem_access_valid (mem: Memory) (p : Ptr) : Prop :=
-  let a := find_array mem p in
+Definition mem_access_valid (mem: Memory) (base : uintptr) (offset : uintptr) : Prop :=
+  let a := find_array mem base in
   let l := match a with
   | Some a' => (Pos.of_nat (len a'))
   | None => 1%positive
   end in
-  (a <> None) /\ ((Pos.ltb (ptr_off p) l) = true).
-
-Ltac mavtac :=
-  match goal with
-    m : Memory,
-    p : Ptr,
-    H : mem_access_valid _ _
-    |- _ =>
-      destruct H as [Hoptinj Hoffset];
-      destruct (find_array m p) eqn:Harray;
-      try congruence;
-      unfold st_mem; unfold st_mem'; unfold st_arr;
-      try rewrite Harray; try rewrite Hoffset
-  end.
+  (a <> None) /\ ((Pos.ltb (uint_to_pos offset) l) = true).
 
 (* random lemma I felt like proving *)
+Ltac isi := intros; split; intros.
 Lemma valid_st_lemma:
-  forall (mem : Memory) (p : Ptr) (v : uint8),
-  mem_access_valid mem p ->
-  (st_mem' mem p v) <> None.
+  forall (mem : Memory) (base : uintptr) (offset : uintptr) (v : uint8),
+  mem_access_valid mem base offset <->
+  (st_mem' mem base offset v) <> None.
 Proof.
-  intros.
-  mavtac.
-  discriminate.
+  isi.
+  - destruct H as [Ha Ho].
+    unfold st_mem'.
+    destruct (find_array mem base0); try (exfalso; congruence).
+    unfold st_arr. rewrite Ho. discriminate.
+  - unfold mem_access_valid.
+    unfold st_mem' in H.
+    destruct (find_array mem base0); try (exfalso; congruence).
+    split; try discriminate.
+    destruct (Pos.ltb (uint_to_pos offset) (Pos.of_nat (len a))) eqn:Hlt; try reflexivity.
+    unfold st_arr in H.
+    rewrite Hlt in H.
+    exfalso. congruence.
+Qed.
+
+Lemma still_valid_lemma:
+  forall (mem : Memory) (base : uintptr) (offset : uintptr) (v : uint8),
+  mem_access_valid mem base offset <->
+  mem_access_valid (st_mem mem base offset v) base offset.
+Proof.
+  isi; unfold mem_access_valid in *; destruct H as [Ha Ho].
+  - split; unfold st_mem, st_mem';
+    destruct (find_array mem base0); try congruence;
+    unfold st_arr;
+    rewrite Ho; unfold find_array;
+    rewrite PMap.gss; try discriminate.
+    simpl. assumption.
+  - split.
+    + unfold st_mem, st_mem' in *.
+      destruct (find_array mem base0) eqn:Hp; try congruence.
+    + unfold st_mem, st_mem' in *.
+      destruct (find_array mem base0) eqn:Hp.
+      * destruct (st_arr a offset v) eqn:Hst.
+      -- destruct (find_array (PMap.set (uint_to_pos base0) (Some a0) mem) base0) eqn:Ha1.
+      ++ unfold find_array in Ha1.
+         rewrite PMap.gss in Ha1.
+         injection Ha1 as Ha1.
+         rewrite <- Ha1 in Ho.
+         unfold st_arr in Hst.
+         destruct ((uint_to_pos offset <? Pos.of_nat (len a))%positive); try reflexivity.
+         exfalso. congruence.
+      ++ exfalso. congruence.
+      -- rewrite Hp in Ho. assumption.
+      * rewrite Hp in Ho. assumption.
 Qed.
 
 (* read after write lemmas *)
 Lemma raw_same_address:
-  forall (mem : Memory) (p : Ptr) (v : uint8),
-  mem_access_valid mem p ->
-  ld_mem (st_mem mem p v) p = Some v.
-Proof.
-  intros.
-  mavtac.
-  unfold ld_mem. unfold find_array. unfold ld_arr.
-  rewrite PMap.gss. simpl. rewrite PMap.gss.
-  reflexivity.
+  forall (mem : Memory) (base : uintptr) (offset : uintptr) (v : uint8),
+  mem_access_valid mem base offset <->
+  ld_mem (st_mem mem base offset v) base offset = Some v.
+Proof with try congruence.
+  intros; split; intros.
+  - assert (mem_access_valid (st_mem mem base0 offset v) base0 offset). {
+      apply still_valid_lemma. assumption.
+    }
+    destruct H as [Ha Ho].
+    destruct H0 as [Ha' Ho'].
+    destruct (find_array mem base0) eqn:Hp...
+    destruct (find_array (st_mem mem base0 offset v) base0) eqn:Hp'...
+    unfold ld_mem.
+    destruct (find_array (st_mem mem base0 offset v) base0) eqn:Hp''...
+    unfold ld_arr.
+    injection Hp' as Hp'. rewrite Hp'.
+    destruct ((uint_to_pos offset <? Pos.of_nat (len a0))%positive)...
+    rewrite Hp' in Hp''.
+    unfold find_array in Hp''.
+    unfold st_mem, st_mem' in Hp''.
+    rewrite Hp in Hp''.
+    unfold st_arr in Hp''.
+    rewrite Ho in Hp''.
+    rewrite PMap.gss in Hp''.
+    injection Hp'' as Hp''.
+    rewrite <- Hp''. simpl.
+    rewrite PMap.gss. reflexivity.
+  - unfold mem_access_valid. split.
+    + unfold ld_mem in H.
+      destruct (find_array mem base0) eqn:Hp...
+      unfold st_mem, st_mem' in H.
+      repeat rewrite Hp in H.
+      exfalso. congruence.
+    + unfold ld_mem, ld_arr in H.
+      unfold st_mem, st_mem', st_arr in H.
+      destruct (find_array mem base0) eqn:Hp.
+      * destruct ((uint_to_pos offset <? Pos.of_nat (len a))%positive) eqn:Ho...
+        rewrite Hp in H.
+        rewrite Ho in H.
+        exfalso. congruence.
+      * rewrite Hp in H. exfalso. congruence.
 Qed.
 Lemma raw_different_address:
-  forall (mem : Memory) (p1 p2 : Ptr) (v : uint8),
-  p1 <> p2 ->
-  ld_mem mem p1 = ld_mem (st_mem mem p2 v) p1.
+  forall (mem : Memory) (b1 b2 : uintptr) (o1 o2 : uintptr) (v : uint8),
+  (o1 <> o2 \/ b1 <> b2) ->
+  ld_mem mem b1 o1 = ld_mem (st_mem mem b2 o2 v) b1 o1.
 Proof with try congruence; try discriminate; try reflexivity.
   intros.
-  unfold st_mem. unfold st_mem'.
-  destruct (find_array mem p2) eqn:Hp2...
-  destruct (st_arr a p2 v) eqn:Ha2'...
-
-  unfold ld_mem.
-  unfold find_array.
-  destruct (Pos.eqb (ptr_base p1) (ptr_base p2)) eqn:Heq.
-  - rewrite Pos.eqb_eq in Heq.
-    rewrite Heq.
-    rewrite PMap.gss.
-    unfold ld_arr.
-    unfold st_arr in Ha2'.
-    unfold find_array in Hp2. rewrite Hp2.
-    destruct (Pos.ltb (ptr_off p2) (Pos.of_nat (len a))) eqn:Hp2l...
+  unfold st_mem, st_mem'.
+  destruct (find_array mem b2) eqn:Hp2...
+  destruct (st_arr a o2 v) eqn:Ha2'...
+  unfold ld_mem, find_array.
+  destruct H.
+  - unfold st_arr in Ha2'.
+    destruct (Pos.ltb (uint_to_pos o2) (Pos.of_nat (len a))) eqn:Hltb...
     injection Ha2' as Ha2'.
-    rewrite <- Ha2'. simpl.
-    rewrite PMap.gso...
-    destruct p1. destruct p2. simpl in *.
-    unfold ptr_off. unfold ptr_base in Heq.
-    unfold idx_to_key. unfold idx_to_key in Heq.
-    apply Nat2Pos.inj in Heq; try rewrite Nat.add_1_r...
-    apply Nat.add_cancel_r in Heq.
-    rewrite Heq in H.
-    destruct (offset =? offset0) eqn:Hoff.
-    + apply Nat.eqb_eq in Hoff.
-      rewrite Hoff.
-      congruence.
-    + apply Nat.eqb_neq in Hoff.
-      intro Hcontra.
-      apply Nat2Pos.inj in Hcontra; try rewrite Nat.add_1_r...
-      rewrite Nat.add_1_r in Hcontra. injection Hcontra as Hcontra.
-      contradiction.
-  - rewrite Pos.eqb_neq in Heq.
-    rewrite PMap.gso...
-Qed.
+    destruct (Pos.eq_dec (uint_to_pos b1) (uint_to_pos b2)) as [Hbeq | Hbneq].
+    + repeat rewrite Hbeq. rewrite PMap.gss.
+      unfold find_array in Hp2.
+      rewrite Hp2.
+      unfold ld_arr.
+      rewrite <- Ha2'; simpl.
+      rewrite PMap.gso...
+      unfold uint_to_pos.
+      admit.
+      (* intro Heq.
+      apply Nat2Pos.inj in Heq.
+      * unfold Z.to_nat in Heq.
+        destruct  *)
+    + rewrite PMap.gso...
+  - rewrite PMap.gso...
+    admit.
+Admitted.
 
-(* Case 2 Example *)
-Inductive Value : Type :=
-| Numeric (val: uint8)
-| Pointer (val : Ptr)
-| NilVal.
-Definition Registers : Type := PMap.t Value.
-Record Machine := {
-  registers: Registers;
-  memory: Memory
+(* Toy Grammar *)
+(* Values *)
+From MyProject Require Import CrVal.
+Inductive RegArg : Type :=
+| Reg (x : positive).
+Definition reg' (r : RegArg) : positive :=
+  match r with
+  | Reg x => x
+  end.
+
+(* Operators *)
+Inductive Op : Type :=
+  (*  *)
+  (* creates an array in memory *)
+| Alloc (base nbyte : nat)
+  (* dst_reg = v *)
+| SetVal (dst_reg : RegArg) (v : CrVal)
+  (* dst_reg = src_reg *)
+| SetReg (dst_reg src_reg : RegArg)
+  (* dst_reg = *src_reg *)
+| LdReg (dst_reg src_reg : RegArg)
+  (* *dst_reg = v *)
+| StVal (dst_reg : RegArg) (v : CrVal)
+  (* *dst_reg = src_reg *)
+| StReg (dst_reg src_reg : RegArg)
+  (* *dst_reg = *src_reg *)
+| IStReg (dst_reg src_reg : RegArg)
+  (* dst_reg = src_reg + v *)
+| AddVal (dst_reg src_reg : RegArg) (v : CrVal)
+  (* dst_reg = src_reg1 + src_reg2 *)
+| AddReg (dst_reg src_reg1 src_reg2 : RegArg).
+
+Record MachineState := {
+  reg_state : PMap.t CrVal;
+  mem_state : Memory;
 }.
 
-Definition TabulaRasa : Machine := {|
-  registers := PMap.init NilVal;
-  memory := PMap.init None
-|}.
+Definition Interp : Type :=
+  MachineState -> MachineState.
+Definition Program : Type :=
+  list Op.
 
-Definition alloc (m : Machine) (base nbyte : nat) : Machine := {|
-  registers := registers m;
-  memory := PMap.set (Pos.of_nat (base+1)) (Some {|
+Definition get_reg (m : MachineState) (r : RegArg) : CrVal :=
+  (reg_state m) !! (reg' r).
+Transparent get_reg.
+Definition x_reg (m : MachineState) (r : RegArg) : CrVal :=
+  match get_reg m r with
+  | CrPtr b o =>
+    match ld_mem (mem_state m) b o with
+    | Some v => CrInt v
+    | None => CrNil
+    end
+  | _ => CrNil
+  end.
+Transparent x_reg.
+Definition alloc (base nbyte : nat) (m : MachineState) : MachineState := {|
+  reg_state := reg_state m;
+  mem_state := PMap.set (Pos.of_nat (base+1)) (Some {|
     base := base;
     len := nbyte;
     bytes := PMap.init None
-  |}) (memory m)
+  |}) (mem_state m);
 |}.
-Definition get_reg (m : Machine) (i : positive) : Value :=
-  (registers m) !! i.
-Definition x_reg (m : Machine) (i : positive) : Value :=
-  match get_reg m i with
-  | Pointer p => match ld_mem (memory m) p with
-    | Some v => Numeric v
-    | None => NilVal
-    end
-  | _ => NilVal
-  end.
-Definition set_reg (m : Machine) (i : positive) (v : Value) : Machine := {|
-  registers := PMap.set i v (registers m);
-  memory := memory m
+Transparent alloc.
+Definition set_val (dst_reg : RegArg) (v : CrVal) (m : MachineState) : MachineState := {|
+  reg_state := PMap.set (reg' dst_reg) v (reg_state m);
+  mem_state := mem_state m;
 |}.
-
-(* t = *f *)
-Definition ld_reg (m : Machine) (f t : positive) : Machine :=
-  match get_reg m f with
-  | Pointer p =>
-    match ld_mem (memory m) p with
-    | Some res => set_reg m t (Numeric res)
-    | None => m
-    end
-  | _ => m
-  end.
-(* *t = f *)
-Definition st_reg (m : Machine) (f t : positive) : Machine :=
-  match (get_reg m t), (get_reg m f) with
-  | Pointer p, Numeric v => {|
-      registers := registers m;
-      memory := st_mem (memory m) p v
+Transparent set_val.
+Definition set_reg (dst_reg src_reg : RegArg) (m : MachineState) : MachineState := {|
+  reg_state := PMap.set (reg' dst_reg) ((reg_state m) !! (reg' src_reg)) (reg_state m);
+  mem_state := mem_state m;
+|}.
+Definition ld_reg (dst_reg src_reg : RegArg) (m : MachineState) : MachineState :=
+  let ld_val := x_reg m src_reg in {|
+  reg_state := PMap.set (reg' dst_reg) ld_val (reg_state m);
+  mem_state := mem_state m;
+|}.
+Transparent ld_reg.
+Definition st_val (dst_reg : RegArg) (v : CrVal) (m : MachineState) : MachineState :=
+  match (reg_state m) !! (reg' dst_reg), v with
+  | CrPtr b o, CrInt x => {|
+      reg_state := reg_state m;
+      mem_state := st_mem (mem_state m) b o x;
     |}
   | _, _ => m
   end.
-  
-Definition add_ (v1 v2 : Value) : Value :=
-  match v1, v2 with
-  | Numeric x, Numeric y => Numeric (Integers.add x y)
-  | Pointer (Address x y), Numeric z =>
-    Pointer (Address x (y + (Z.to_nat (unsigned z))))
-  | _, _ => NilVal
+Transparent st_val.
+Definition st_reg (dst_reg src_reg : RegArg) (m : MachineState) : MachineState :=
+  match (reg_state m) !! (reg' dst_reg), (reg_state m) !! (reg' src_reg) with
+  | CrPtr b o, CrInt x => {|
+      reg_state := reg_state m;
+      mem_state := st_mem (mem_state m) b o x;
+    |}
+  | _, _ => m
   end.
+Transparent st_reg.
+Definition ist_reg (dst_reg src_reg : RegArg) (m : MachineState) : MachineState :=
+  match (reg_state m) !! (reg' dst_reg), (reg_state m) !! (reg' src_reg) with
+  | CrPtr b' o', CrPtr b o => match ld_mem (mem_state m) b o with
+    | Some v => {|
+        reg_state := reg_state m;
+        mem_state := st_mem (mem_state m) b' o' v;
+      |}
+    | None => m
+    end
+  | _, _ => m
+  end.
+Transparent ist_reg.
+Definition add_val (dst_reg src_reg : RegArg) (v : CrVal) (m : MachineState) : MachineState :=
+  set_val dst_reg match (reg_state m) !! (reg' src_reg), v with
+  | CrInt x, CrInt y => CrInt (Integers.add x y)
+  | CrPtr x y, CrInt z =>
+    let z' : uintptr := repr (intval z) in
+    CrPtr x (Integers.add y z')
+  | _, _ => CrNil
+  end m.
+Transparent add_val.
+Definition add_reg (dst_reg src_reg1 src_reg2 : RegArg) (m : MachineState) : MachineState :=
+  set_val dst_reg match (reg_state m) !! (reg' src_reg1), (reg_state m) !! (reg' src_reg2) with
+  | CrInt x, CrInt y => CrInt (Integers.add x y)
+  | CrPtr x y, CrInt z =>
+    let z' : uintptr := repr (intval z) in
+    CrPtr x (Integers.add y z')
+  | _, _ => CrNil
+  end m.
+Transparent add_reg.
 
-Definition m' :=
-  (* initialize *)
-  let m0 := TabulaRasa in
-  (* alloc 128 bytes @ 0 *)
-  let m1 := alloc m0 0 128 in
-  (* u8* r1 = 0x0 *)
-  let m2 := set_reg m1 1 (Pointer (Address 0 0)) in
-  (* *0x0 = 67 *)
-  let m3 := {|
-    registers := registers m2;
-    memory := st_mem (memory m2) (Address 0 0) (repr 67)
-  |} in
-  m3.
+Definition apply_op (op : Op) (m : MachineState) : MachineState :=
+  match op with
+  | Alloc b n => alloc b n
+  | SetVal d v => set_val d v
+  | SetReg d s => set_reg d s
+  | LdReg d s => ld_reg d s
+  | StVal d v => st_val d v
+  | StReg d s => st_reg d s
+  | IStReg d s => ist_reg d s
+  | AddVal d s v => add_val d s v
+  | AddReg d s1 s2 => add_reg d s1 s2
+  end m.
 
-Definition prog_1 :=
-  (* Example Program *)
-  (* r3 = *r1 *)
-  let m4 := ld_reg m' 1 3 in
-  (* r6 = 10 *)
-  let m5 := set_reg m4 6 (Numeric (repr 10)) in
-  (* r7 = r1 *)
-  let m6 := set_reg m5 7 (get_reg m5 1) in
-  (* *r7 = r6 *)
-  let m7 := st_reg m6 6 7 in
-  (* r5 = r1 *)
-  let m8 := set_reg m7 5 (get_reg m7 1) in
-  (* r4 = *r5 *)
-  let m9 := ld_reg m8 5 4 in
-  (* r2 = r3 + r4 *)
-  let ma := set_reg m9 2 (add_
-    (get_reg m9 3)
-    (get_reg m9 4)) in
-  get_reg ma 2.
+Fixpoint compile' (p : Program) (m : MachineState) : MachineState :=
+  match p with
+  | [] => m
+  | x :: xs => compile' xs (apply_op x m)
+  end.
+Definition compile (p : Program) : Interp :=
+  compile' p.
 
-Definition prog_2 :=
-  (* r3 = *r1 *)
-  let m4 := ld_reg m' 1 3 in
-  (* r6 = 10 *)
-  let m5 := set_reg m4 6 (Numeric (repr 10)) in
-  (* r2 = r3 + r6 *)
-  let m6 := set_reg m5 2 (add_
-    (get_reg m5 6)
-    (get_reg m5 3)) in
-  get_reg m6 2.
+From MyProject Require Import SmtExpr.
+Definition check_registers_and_memory (s1 s2 : MachineState)
+  (reg_list : list RegArg) (mem_list : list (uintptr * uintptr)) : SmtBoolExpr :=
+  SmtBoolNot (SmtBoolAnd
+    (List.fold_right
+      (fun r acc => SmtBoolAnd acc (SmtBoolEq
+        (SmtConst (get_reg s1 r))
+        (SmtConst (get_reg s2 r))))
+      SmtTrue reg_list)
+    (List.fold_right (fun p acc =>
+      SmtBoolAnd acc (match p with
+      | (base, offset) =>
+        SmtBoolEq
+          (match ld_mem (mem_state s1) base offset with
+          | Some v => SmtConst (CrInt v)
+          | None => SmtConst CrNil
+          end)
+          (match ld_mem (mem_state s2) base offset with
+          | Some v => SmtConst (CrInt v)
+          | None => SmtConst CrNil
+          end)
+      end))
+      SmtTrue mem_list)
+  ).
 
-Example p1_p2_eq:
-  prog_1 = prog_2.
+From MyProject Require Import SmtTypes.
+From MyProject Require Import SmtQuery.
+Definition eq_checker (s : MachineState)
+  (p1 p2 : Program)
+  (reg_list : list RegArg) (mem_list : list (uintptr * uintptr)) : SmtResult :=
+  let s1 := compile p1 s in
+  let s2 := compile p2 s in
+  smt_query (check_registers_and_memory s1 s2 reg_list mem_list).
+
+Record ProgramOutput := {
+  out_reg : list RegArg;
+  out_mem : list Ptr;
+}.
+
+Definition get_output (p : Program) (o : ProgramOutput) (m : MachineState) : list Value * list Value :=
+  let m' := (compile p) m in
+  (* for each number in (out_reg o), map get_reg onto m' *)
+  let reg_vals := List.map (fun r => (reg_state m') !! (reg' r)) (out_reg o) in
+  let mem_vals := List.map (fun p =>
+    match ld_mem (mem_state m') p with
+    | Some v => VInt v
+    | None => VNil
+    end
+  ) (out_mem o) in
+  (reg_vals, mem_vals).
+
+Definition programs_eq (p1 p2 : Program) (out : ProgramOutput) :=
+  forall (m : MachineState),
+  get_output p1 out m = get_output p2 out m.
+
+Definition TabulaRasa : MachineState := {|
+  reg_state := PMap.init VNil;
+  mem_state := PMap.init None
+|}.
+
+Definition mx : MachineState := {|
+  reg_state := PMap.set 1 (VPtr (Address 0 0)) (PMap.init VNil);
+  mem_state := PMap.set (Pos.of_nat 1) (Some {|
+    base := 0;
+    len := 1024;
+    bytes := PMap.set 1 (Some (repr 10)) (PMap.init None)
+  |}) (PMap.init None)
+|}.
+
+Definition p1_v1 : Program := [
+  LdReg  (Reg 3) (Reg 1); (* r3 = *r1 *)
+  SetVal (Reg 6) (VInt (repr 10)); (* r6 = 10 *)
+  SetReg (Reg 7) (Reg 1); (* r7 = r1 *)
+  StReg  (Reg 7) (Reg 6); (* *r7 = r6 *)
+  SetReg (Reg 5) (Reg 1); (* r5 = r1 *)
+  LdReg  (Reg 4) (Reg 5); (* r4 = *r5 *)
+  AddReg (Reg 2) (Reg 3) (Reg 4) (* r2 = r3 + r4 *)
+].
+Definition p1_v2 : Program := [
+  LdReg  (Reg 2) (Reg 1); (* r2 = *r1 *)
+  AddVal (Reg 2) (Reg 2) (VInt (repr 10)) (* r2 = r2 + 10 *)
+].
+Definition p1_out : ProgramOutput := {|
+  out_reg := [Reg 2; Reg 17];
+  out_mem := [(Address 100 100)]
+|}.
+
+Definition check_registers_and_memory (s1 s2 : MachineState)
+  (out_list : ProgramOutput)
+
+Compute (get_output p1_v1 p1_out mx).
+Compute get_output p1_v2 p1_out mx.
+
+(* memory operators don't change register state *)
+Lemma alloc_is_regnop : forall base nbyte m,
+  reg_state (alloc base nbyte m) = reg_state m.
+Proof. intros. reflexivity. Qed.
+Lemma st_val_is_regnop : forall dst v m,
+  reg_state (st_val dst v m) = reg_state m.
+Proof. intros. unfold st_val. destruct ((reg_state m) !! (reg' dst)), v; reflexivity. Qed.
+Lemma st_reg_is_regnop : forall dst src m,
+  reg_state (st_reg dst src m) = reg_state m.
+Proof. intros. unfold st_reg. destruct ((reg_state m) !! (reg' dst)), ((reg_state m) !! (reg' src)); reflexivity. Qed.
+Lemma ist_reg_is_regnop : forall dst src m,
+  reg_state (ist_reg dst src m) = reg_state m.
+Proof. intros. unfold ist_reg. destruct ((reg_state m) !! (reg' dst)), ((reg_state m) !! (reg' src)); try reflexivity. destruct (ld_mem (mem_state m) p0); reflexivity. Qed.
+
+(* register operators don't change memory state *)
+Lemma set_val_is_memnop : forall dst v m,
+  mem_state (set_val dst v m) = mem_state m.
+Proof. intros. reflexivity. Qed.
+Lemma set_reg_is_memnop : forall dst src m,
+  mem_state (set_reg dst src m) = mem_state m.
+Proof. intros. reflexivity. Qed.
+Lemma ld_reg_is_memnop : forall dst src m,
+  mem_state (ld_reg dst src m) = mem_state m.
+Proof. intros. reflexivity. Qed.
+Lemma add_val_is_memnop : forall dst src v m,
+  mem_state (add_val dst src v m) = mem_state m.
+Proof. intros. reflexivity. Qed.
+Lemma add_reg_is_memnop : forall dst src1 src2 m,
+  mem_state (add_reg dst src1 src2 m) = mem_state m.
+Proof. intros. reflexivity. Qed.
+
+(* register operators don't affect other registers *)
+Lemma set_val_diff : forall r1 r2 v m,
+  r1 <> reg' r2 -> (reg_state (set_val r2 v m)) !! r1 = (reg_state m) !! r1.
+Proof. intros. simpl. rewrite PMap.gso; try reflexivity. assumption. Qed.
+Lemma set_reg_diff : forall r1 r2 src m,
+  r1 <> reg' r2 -> (reg_state (set_reg r2 src m)) !! r1 = (reg_state m) !! r1.
+Proof. intros. simpl. rewrite PMap.gso; try reflexivity. assumption. Qed.
+Lemma ld_reg_diff : forall r1 r2 src m,
+  r1 <> reg' r2 -> (reg_state (ld_reg r2 src m)) !! r1 = (reg_state m) !! r1.
+Proof. intros. simpl. rewrite PMap.gso; try reflexivity. assumption. Qed.
+Lemma add_val_diff : forall r1 r2 src v m,
+  r1 <> reg' r2 -> (reg_state (add_val r2 src v m)) !! r1 = (reg_state m) !! r1.
+Proof. intros. unfold add_val. apply set_val_diff. assumption. Qed.
+Lemma add_reg_diff : forall r1 r2 src1 src2 m,
+  r1 <> reg' r2 -> (reg_state (add_reg r2 src1 src2 m)) !! r1 = (reg_state m) !! r1.
+Proof. intros. unfold add_reg. apply set_val_diff. assumption. Qed.
+
+(* apply register operator *)
+Lemma ld_reg_same : forall r src m,
+  (reg_state (ld_reg (Reg r) src m)) !! r = x_reg m src.
 Proof.
-  unfold prog_1. unfold prog_2.
-  unfold get_reg. simpl.
-  repeat rewrite PMap.gss.
-  unfold add.
-  simpl.
-  reflexivity.
+  intros. simpl. rewrite PMap.gss. reflexivity.
 Qed.
